Terms/Perm.v
@@ -8,6 +8,7 @@ Require Import Top.FinSet.FPCard.
 Require Import Top.FinSet.NatMap.
 Require Import Top.FinSet.ProjSet.
 Require Import Top.Terms.Term.
+Require Import Top.Terms.Subst.
 
 Set Implicit Arguments.
 
@@ -31,7 +32,7 @@ Section var_subst.
       would hope that a [var_subst] induces one, and it does. *)
 
   Lemma fin_subst_var_subst s
-    : fin_subst (var_subst_subst s).
+    : fin_subst L (var_subst_subst s).
   Proof.
     destruct s as [ f finH ]; simpl.
     apply (compose_fin_mod decV decV (decTerm decV decF));
