Terms/Subst.v
@@ -1,0 +1,273 @@
+(** This library describes a [fin_subst] (called a substitution in
+    Eder's paper), which is a rule for substituting terms for
+    variables in a term. *)
+
+Require Import Lists.List.
+
+Require Import Top.FinSet.FinMod.
+Require Import Top.FinSet.ListMod.
+
+Require Import Top.Terms.Term.
+Require Import Top.Terms.VecUtils.
+
+(** * Substitutions
+
+    Eder's paper talks about substitutions as if they are
+    endomorphisms on Term, but he is only interested in the
+    endomorphisms that come about from actual substitutions: maps
+    from variables to terms which may or may not themselves be
+    variables.
+
+    Let's start by defining the induced endomorphism on Term that
+    comes from a substitution. *)
+Section subst.
+  Variable L : lType.
+
+  Definition Subst := Term.V L -> Term L.
+
+  Fixpoint subst_endo (s : Subst) (t : Term L) : Term L :=
+    match t with
+    | varTerm _ v => s v
+    | funTerm f ts => funTerm f (VectorDef.map (subst_endo s) ts)
+    end.
+
+  (** One map from [V] to [Term] is [varTerm] (the [Term] constructor
+      for variable names). This should induce the identity. The point
+      is that the induced endomorphism is exactly filling in each "v"
+      with "v" again.  *)
+
+  Lemma subst_endo_varTerm {t}
+    : subst_endo (varTerm L) t = t.
+  Proof.
+    revert t; apply Term_ind'; try reflexivity.
+    intros f ts allH.
+    unfold subst_endo; fold subst_endo.
+    apply f_equal.
+    induction ts as [ | t n ts IH ]; try reflexivity.
+    destruct allH as [ tH tsH ].
+    specialize (IH tsH); clear tsH.
+    unfold VectorDef.map;
+      fold (@VectorDef.map (Term L) _ (subst_endo (varTerm L))).
+    rewrite IH, tH.
+    exact eq_refl.
+  Qed.
+
+  (** Another fact we might want to know about these induced
+      endomorphisms is extensionality. That is, if two substitutions
+      have the same values on all of [V] then their induced
+      endomorphisms have the same values on all of [Term]. (This sort
+      of messing around is needed because functions aren't extensional
+      in Coq). *)
+
+  Lemma subst_endo_ex {s s' t}
+    : (forall v, s v = s' v) -> subst_endo s t = subst_endo s' t.
+  Proof.
+    intro eqH.
+    revert t; apply Term_ind'.
+    - intro v; specialize (eqH v). tauto.
+    - intros f ts allH.
+      unfold subst_endo; fold subst_endo.
+      apply f_equal.
+      apply vec_map_ext.
+      exact allH.
+  Qed.
+
+  (** Obviously, we can't compose substitutions directly (because they
+      are maps [V -> Term]). However, we can compose their induced
+      endomorphisms and then restrict back to variables by composing
+      with [varTerm]. *)
+
+  Definition comp_subst (sigma tau : Subst) : Subst :=
+    fun v => subst_endo sigma (tau v).
+
+  (** Fortunately, given the name, [comp_subst] is indeed the right
+      notion of composition of substitutions. In fact, if you compose
+      the induced endomorphisms from two substitutions, you get the
+      same thing as if you use [comp_subst] to compose the
+      substitutions and then induce the endomorphism. *)
+
+  Lemma compose_subst_endo (sigma tau : Subst) (t : Term L)
+    : subst_endo sigma (subst_endo tau t) =
+      subst_endo (comp_subst sigma tau) t.
+  Proof.
+    revert t; apply Term_ind'; try tauto.
+    intros f ts IH.
+    unfold subst_endo; fold subst_endo; apply f_equal.
+    rewrite vec_map_map.
+    auto using vec_map_ext.
+  Qed.
+
+  (** As you would hope, [varTerm] is a left and right identity for
+      [comp_subst]. *)
+
+  Lemma comp_subst_idl {sigma v} : comp_subst (varTerm L) sigma v = sigma v.
+  Proof.
+    unfold comp_subst; auto using subst_endo_varTerm.
+  Qed.
+
+  Lemma comp_subst_idr {sigma v} : comp_subst sigma (varTerm L) v = sigma v.
+  Proof.
+    unfold comp_subst; auto using subst_endo_varTerm.
+  Qed.
+
+  (** Also, unsurprisingly, [comp_subst] is associative. *)
+
+  Lemma comp_subst_assoc {s1 s2 s3 v}
+    : comp_subst s1 (comp_subst s2 s3) v = comp_subst (comp_subst s1 s2) s3 v.
+  Proof.
+    unfold comp_subst; simpl.
+    generalize (s3 v); clear s3 v.
+    apply Term_ind'; try reflexivity.
+    intros f ts IH.
+    unfold subst_endo at 2; fold subst_endo.
+    unfold subst_endo at 1; fold subst_endo.
+    unfold subst_endo at 3; fold subst_endo.
+    apply f_equal.
+    rewrite vec_map_map.
+    apply vec_map_ext.
+    exact IH.
+  Qed.
+
+  (** A technical lemma about extensionality. If we have two
+      factorisations where the factors are extensionally equal, then the
+      composite maps must be too. *)
+
+  Lemma comp_subst_ex {r r' s s'} (v : Term.V L)
+    : (forall v, r v = r' v) ->
+      (forall v, s v = s' v) ->
+      comp_subst r s v = comp_subst r' s' v.
+  Proof.
+    intros rH sH.
+    unfold comp_subst; rewrite sH, (subst_endo_ex rH); auto.
+  Qed.
+
+  (** Define the image of a substitution: the terms that you get when
+      applying the substitution to each variable in [V]. The set is
+      encoded as a predicate. *)
+  Definition subst_im (s : Subst) (t : Term L) : Prop :=
+    exists v, t = s v.
+
+  (** * Finite substitutions
+
+      Now we get to an important definition: [fin_subst]. Eder is only
+      interested in substitutions that map only finitely many
+      variables differently from [varTerm]. In our development, this
+      means that it should be a finite modification of [varTerm]. *)
+
+  Definition fin_subst := fin_mod (varTerm L).
+
+  (** We can construct our first [fin_subst] from varTerm. Since this
+      is a trivial modification of [varTerm], it definitely satisfies
+      the definition. *)
+
+  Lemma fin_subst_varTerm : fin_subst (varTerm L).
+  Proof.
+    apply fin_mod_i.
+  Qed.
+
+  (** It's a bit more difficult to show that [fin_subst] maps are
+      closed under composition (using [comp_subst]). I think that the
+      substitution that induces the composition of two induced
+      endomorphisms is actually easiest to define by concatenating
+      lists, so we start in terms of list maps. *)
+
+  Section fin_comp_subst.
+    Variables sigma tau : Subst.
+    Variable sl tl : list (Term.V L * Term L).
+
+    Hypothesis decV : forall x y : Term.V L, {x = y} + {x <> y}.
+    Hypothesis decF : forall x y : Term.F L, {x = y} + {x <> y}.
+
+    Hypothesis sH : forall v, sigma v = list_map decV (varTerm L) sl v.
+    Hypothesis tH : forall v, tau v = list_map decV (varTerm L) tl v.
+
+    (** A list inducing the correct correct composed map ([compose
+        sigma tau]) is given by first mapping all the variables to
+        where [tau] would send them and then applying the induced map
+        from [sigma] to the resulting term.
+
+        Variables that weren't moved by [tau] get mapped by [sigma],
+        which we can express by shoving them to the end of the
+        list. *)
+
+    Local Definition stl : list (Term.V L * Term L) :=
+      app (map (fun p => (fst p, subst_endo sigma (snd p))) tl)
+          sl.
+
+    Lemma stl_map_v v
+      : list_map decV (varTerm L) stl v = comp_subst sigma tau v.
+    Proof.
+      specialize (tH v).
+      unfold comp_subst, subst_endo, stl.
+      set (pmap := (fun p => (fst p, subst_endo sigma (snd p)))).
+      revert tau tH.
+      induction tl as [ | p tl' IH ].
+      - intros; rewrite tH; simpl; auto.
+      - intros tau tH.
+        clear tl; rename tl' into tl.
+        rewrite (map_cons pmap p tl), <- app_comm_cons.
+        destruct p as [ v' sv' ].
+        destruct (decV v' v) as [ veqH | vneH ].
+        + rewrite veqH in *; clear v' veqH.
+          simpl in tH; rewrite upd_map_at in tH.
+          unfold pmap; simpl; rewrite upd_map_at.
+          rewrite tH. tauto.
+        + unfold pmap at 1; simpl.
+          rewrite (upd_map_not_at decV _ _ (not_eq_sym vneH)).
+          simpl in tH.
+          rewrite (upd_map_not_at decV _ _ (not_eq_sym vneH)) in tH.
+          apply IH.
+          apply tH.
+    Qed.
+  End fin_comp_subst.
+
+  (** Since we worked in terms of list maps, we now must use the
+      correspondence between those and finite mods to conclude that
+      the composition of two finite substitutions is itself finite
+      (assuming that equality of terms is decidable) *)
+
+  Lemma fin_subst_comp sigma tau
+    : (forall x y : Term.V L, {x = y} + {x <> y}) ->
+      (forall x y : Term.F L, {x = y} + {x <> y}) ->
+      fin_subst sigma -> fin_subst tau -> fin_subst (comp_subst sigma tau).
+  Proof.
+    unfold fin_subst at 1 2.
+    intros decV decF fmS fmT.
+    set (decT := (decTerm decV decF)).
+    destruct (fin_mod_is_list_map decV decT fmS) as [ sl slH ].
+    destruct (fin_mod_is_list_map decV decT fmT) as [ tl tlH ].
+    destruct slH as [ slH _ ].
+    destruct tlH as [ tlH _ ].
+    apply (fin_mod_ex _ _ _ _
+                      (fun x => eq_refl (varTerm L x))
+                      (stl_map_v sigma tau sl tl decV slH tlH)).
+    apply (fin_mod_list_map decV _ decT).
+  Qed.
+
+  (** Finally, we show that restricting a finite substitution to
+      variables satisfying some predicate doesn't stop it being
+      finite. *)
+
+  Lemma fin_subst_restrict
+        {s P} (decP : forall v : Term.V L, {P v} + {~ P v})
+    : fin_subst s -> fin_subst (restrict_map (varTerm L) P decP s).
+  Proof.
+    unfold fin_subst.
+    apply restrict_preserves_fin_mod.
+  Qed.
+
+  Lemma term_height_subst {s}
+    : forall t, term_height t <= term_height (subst_endo s t).
+  Proof.
+    apply Term_ind'; auto using le_0_n.
+    intros.
+    apply le_n_S; fold (subst_endo s); fold term_height.
+    auto using vec_max_at_map_le.
+  Qed.
+
+  Lemma term_height_comp_subst {s' s v}
+    : term_height (s v) <= term_height (comp_subst s' s v).
+  Proof.
+    apply term_height_subst.
+  Qed.
+End subst.
